IsaSAT: compile

Weidenbach_Book/IICF_Array_List32.thy
@@ -374,18 +374,4 @@ proof -
       simp flip: nat_of_uint32_le_iff)
 qed
 
-definition arl_nat_of_uint64_conv :: \<open>nat list \<Rightarrow> nat list\<close> where
-\<open>arl_nat_of_uint64_conv S = S\<close>
-
-lemma arl_nat_of_uint64_conv_alt_def:
-  \<open>arl_nat_of_uint64_conv = map nat_of_uint64_conv\<close>
-  unfolding nat_of_uint64_conv_def arl_nat_of_uint64_conv_def by auto
-
-lemma arl_nat_of_uint64_conv_hnr[sepref_fr_rules]:
-  \<open>(arl_nat_of_uint64_code, (RETURN \<circ> arl_nat_of_uint64_conv))
-    \<in> (arl_assn uint64_nat_assn)\<^sup>k \<rightarrow>\<^sub>a arl_assn nat_assn\<close>
-  using arl_nat_of_uint64_code.refine[unfolded array_nat_of_uint64_def,
-    FCOMP op_map_map_rel[unfolded convert_fref]] unfolding arl_nat_of_uint64_conv_alt_def
-  by simp
-
 end
