Weidenbach_Book/IICF_Array_List64.thy
@@ -369,4 +369,25 @@ proof -
      split: prod.splits if_splits)
 qed
 
+definition arl_nat_of_uint64_conv :: \<open>nat list \<Rightarrow> nat list\<close> where
+\<open>arl_nat_of_uint64_conv S = S\<close>
+
+lemma arl_nat_of_uint64_conv_alt_def:
+  \<open>arl_nat_of_uint64_conv = map nat_of_uint64_conv\<close>
+  unfolding nat_of_uint64_conv_def arl_nat_of_uint64_conv_def by auto
+
+sepref_definition arl_nat_of_uint64_code
+  is array_nat_of_uint64
+  :: \<open>(arl_assn uint64_nat_assn)\<^sup>k \<rightarrow>\<^sub>a arl_assn nat_assn\<close>
+  unfolding op_map_def array_nat_of_uint64_def arl_fold_custom_replicate
+  apply (rewrite at \<open>do {let _ = \<hole>; _}\<close> annotate_assn[where A=\<open>arl_assn nat_assn\<close>])
+  by sepref
+
+lemma arl_nat_of_uint64_conv_hnr[sepref_fr_rules]:
+  \<open>(arl_nat_of_uint64_code, (RETURN \<circ> arl_nat_of_uint64_conv))
+    \<in> (arl_assn uint64_nat_assn)\<^sup>k \<rightarrow>\<^sub>a arl_assn nat_assn\<close>
+  using arl_nat_of_uint64_code.refine[unfolded array_nat_of_uint64_def,
+    FCOMP op_map_map_rel[unfolded convert_fref]] unfolding arl_nat_of_uint64_conv_alt_def
+  by simp
+
 end
